DomainTypedLispFormalization/CoreSyntax.lean
@@ -20,32 +20,40 @@ inductive Pattern where
   | ctor (name : Name) (fields : List Pattern)
   deriving Repr
 
-mutual
-  inductive Expr where
-    | var (name : Name)
-    | symbol (value : Name)
-    | int (value : Int)
-    | bool (value : Bool)
-    | call (name : Name) (args : List Expr)
-    | letE (bindings : List (Name × Expr)) (body : Expr)
-    | ifE (cond : Expr) (thenBranch : Expr) (elseBranch : Expr)
-    | matchE (scrutinee : Expr) (arms : List (Pattern × Expr))
-    deriving Repr
+inductive Expr where
+  | var (name : Name)
+  | symbol (value : Name)
+  | int (value : Int)
+  | bool (value : Bool)
+  | call (name : Name) (args : List Expr)
+  | letE (bindings : List (Name × Expr)) (body : Expr)
+  | ifE (cond : Expr) (thenBranch : Expr) (elseBranch : Expr)
+  | matchE (scrutinee : Expr) (arms : List (Pattern × Expr))
+  deriving Repr
 
-  inductive Term where
-    | var (name : Name)
-    | symbol (value : Name)
-    | int (value : Int)
-    | bool (value : Bool)
-    | ctor (name : Name) (args : List Term)
-    deriving Repr
+inductive Term where
+  | var (name : Name)
+  | symbol (value : Name)
+  | int (value : Int)
+  | bool (value : Bool)
+  | ctor (name : Name) (args : List Term)
+  deriving Repr
 
-  inductive Formula where
-    | triv
-    | pred (name : Name) (args : List Term)
-    | andF (goals : List Formula)
-    | notF (goal : Formula)
-    deriving Repr
-end
+inductive Formula where
+  | triv
+  | pred (name : Name) (args : List Term)
+  | andF (goals : List Formula)
+  | notF (goal : Formula)
+  deriving Repr
+
+structure Atom where
+  pred : Name
+  terms : List Term
+  deriving Repr
+
+structure Rule where
+  head : Atom
+  body : Formula
+  deriving Repr
 
 end DomainTypedLispFormalization
